thir-elab/coq-extraction/Extra_coq_lib.v
@@ -1,0 +1,121 @@
+From Hacspec Require Import Hacspec_Lib MachineIntegers.
+From Coq Require Import ZArith.
+Import List.ListNotations.
+Open Scope Z_scope.
+Open Scope bool_scope.
+Open Scope hacspec_scope.
+
+Definition int_xI {WS : WORDSIZE} (a : int) : int := MachineIntegers.add (MachineIntegers.mul a (repr 2)) MachineIntegers.one.
+Definition int_xO {WS : WORDSIZE} (a : int) : int := MachineIntegers.mul a (repr 2).
+Number Notation int Pos.of_num_int Pos.to_num_int (via positive mapping [[int_xI] => xI, [int_xO] => xO , [MachineIntegers.one] => xH]) : hacspec_scope.
+Notation "0" := (repr O).
+Notation U8_t := int8.
+Notation U8 := id.
+Notation U16_t := int16.
+Notation U16 := id.
+Notation U32_t := int32.
+Notation U32 := id.
+Notation U64_t := int64.
+Notation U64 := id.
+Notation U128_t := int128.
+Notation U128 := id.
+
+Notation " x .[ a ]" := (array_index x a) (at level 40).
+Notation " x .[ i ]<- a" := (array_upd x i a) (at level 40).
+
+Class Addition A := add : A -> A -> A.
+Notation "a .+ b" := (add a b).
+Instance array_add_inst {ws : WORDSIZE} {len: nat} : Addition (nseq (@int ws) len) := { add a b := a array_add b }.
+Instance int_add_inst {ws : WORDSIZE} : Addition (@int ws) := { add a b := MachineIntegers.add a b }.
+
+Class Subtraction A := sub : A -> A -> A.
+Notation "a .- b" := (sub a b).
+Instance array_sub_inst {ws : WORDSIZE} {len: nat} : Subtraction (nseq (@int ws) len) := { sub := array_join_map MachineIntegers.sub }.
+Instance int_sub_inst {ws : WORDSIZE} : Subtraction (@int ws) := { sub a b := MachineIntegers.sub a b }.
+
+Class Multiplication A := mul : A -> A -> A.
+Notation "a .* b" := (mul a b).
+Instance array_mul_inst {ws : WORDSIZE} {len: nat} : Multiplication (nseq (@int ws) len) := { mul a b := a array_mul b }.
+Instance int_mul_inst {ws : WORDSIZE} : Multiplication (@int ws) := { mul a b := MachineIntegers.mul a b }.
+
+Class Xor A := xor : A -> A -> A.
+Notation "a .^ b" := (xor a b).
+
+Instance array_xor_inst {ws : WORDSIZE} {len: nat} : Xor (nseq (@int ws) len) := { xor a b := a array_xor b }.
+Instance int_xor_inst {ws : WORDSIZE} : Xor (@int ws) := { xor a b := MachineIntegers.xor a b }.
+
+Definition new {A : Type} `{Default A} {len} : nseq A len := array_new_ default _.
+Class array_or_seq A len :=
+{ as_seq : seq A ; as_nseq : nseq A len }.
+
+Arguments as_seq {_} {_} array_or_seq.
+Arguments as_nseq {_} {_} array_or_seq.
+Coercion as_seq : array_or_seq >-> seq.
+Coercion as_nseq : array_or_seq >-> nseq.
+
+Instance nseq_array_or_seq {A len} (a : nseq A len) : array_or_seq A len :=
+{ as_seq := array_to_seq a ; as_nseq := a ; }.
+Coercion nseq_array_or_seq : nseq >-> array_or_seq.
+
+Instance seq_array_or_seq {A} `{Default A} (a : seq A) : array_or_seq A (length a) :=
+{ as_seq := a ; as_nseq := array_from_seq _ a ; }.
+Coercion seq_array_or_seq : seq >-> array_or_seq.
+
+Definition update {A : Type}  `{Default A} {len slen} (s : nseq A len) start (start_a : array_or_seq A slen) : nseq A len :=
+array_update (a := A) (len := len) s start (as_seq start_a).
+
+Definition to_le_U32s {A l} := array_to_le_uint32s (A := A) (l := l).
+Axiom to_le_bytes : forall {ws : WORDSIZE} {len}, nseq (@int ws) len -> seq int8.
+Definition from_seq {A : Type}  `{Default A} {len slen} (s : array_or_seq A slen) : nseq A len := array_from_seq _ (as_seq s).
+
+Notation Seq_t := seq.
+Notation len := (fun s => seq_len s : int32).
+
+Notation slice := array_slice.
+Notation new_seq := seq_new.
+Notation num_exact_chunks := seq_num_exact_chunks.
+Notation get_exact_chunk := seq_get_exact_chunk.
+Definition set_chunk
+{a: Type}
+`{Default a}
+{len}
+(s: seq a)
+(chunk_len: nat)
+(chunk_num: nat)
+(chunk: array_or_seq a len) : seq a :=
+seq_set_chunk s chunk_len chunk_num (as_seq chunk).
+Definition set_exact_chunk {a} `{H : Default a} {len} := @set_chunk a H len.
+Notation get_remainder_chunk := seq_get_remainder_chunk.
+Notation "a <> b" := (negb (eqb a b)).
+
+Notation from_secret_literal := nat_mod_from_secret_literal.
+Definition pow2 {m} (x : @int WORDSIZE32) := nat_mod_pow2 m (unsigned x).
+Instance nat_mod_addition {n} : Addition (nat_mod n) := { add a b := a +% b }.
+Instance nat_mod_subtraction {n} : Subtraction (nat_mod n) := { sub a b := a -% b }.
+Instance nat_mod_multiplication {n} : Multiplication (nat_mod n) := { mul a b := a *% b }.
+Definition from_slice {a: Type} `{Default a} {len slen} (x : array_or_seq a slen) := array_from_slice default len (as_seq x).
+Notation zero := nat_mod_zero.
+Notation to_byte_seq_le := nat_mod_to_byte_seq_le.
+Notation U128_to_le_bytes := u128_to_le_bytes.
+Notation from_byte_seq_le := nat_mod_from_byte_seq_le.
+Definition from_literal {m} := nat_mod_from_literal m.
+Notation inv := nat_mod_inv.
+Notation update_start := array_update_start.
+Notation pow := nat_mod_pow_self.
+Notation bit := nat_mod_bit.
+
+Definition int_to_int {ws1 ws2} (i : @int ws1) : @int ws2 := repr (unsigned i).
+Coercion int_to_int : int >-> int.
+Notation push := seq_push.
+Notation Build_secret := secret.
+Notation "a -× b" :=
+(prod a b) (at level 80, right associativity) : hacspec_scope.
+Notation Result_t := (fun '(x,y) => result).
+Axiom TODO_name : Type.
+Notation ONE := nat_mod_one.
+
+Notation nat_mod := GZnZ.znz.
+
+Instance nat_mod_znz_addition {n} : Addition (GZnZ.znz n) := { add a b := a +% b }.
+Instance nat_mod_znz_subtraction {n} : Subtraction (GZnZ.znz n) := { sub a b := a -% b }.
+Instance nat_mod_znz_multiplication {n} : Multiplication (GZnZ.znz n) := { mul a b := a *% b }.
